Vizing/Fan/Defs.lean
@@ -8,27 +8,27 @@ open Graph
 open EdgeColoring
 open Aux
 
-variable {n : Nat} {c : Nat} (G : Graph n) (C : EdgeColoring c G)
+variable {n c : Nat} {G : Graph n} (C : EdgeColoring c G)
 
 @[simp]
 def fan_prop (x : Vertex n) (f₁ f₂ : Vertex n) :=
-  color c G C (x, f₂) ∈ freeColorsOn G C f₁
+  color C (x, f₂) ∈ freeColorsOn C f₁
 
 def colorAx (F : Array (Vertex n)) (x : Vertex n) :=
-  F.toList.Chain' (fan_prop G C x)
+  F.toList.Chain' (fan_prop C x)
 
 structure Fan (x y : Vertex n) where
   val : Array (Vertex n)
   nborsAx : val.toList ⊆ (nbhd G x).val
   nonemptyAx : val ≠ #[]
   firstElemAx : val[0]'(by exact Array.size_pos_iff.mpr nonemptyAx) = y
-  colorAx : colorAx G C val x
+  colorAx : colorAx C val x
   nodupAx : val.toList.Nodup
 
 variable {n c : Nat} {G : Graph n} {C : EdgeColoring c G} {x y : Vertex n}
 
-theorem fan_colored_edges (x y : Vertex n) (F : Fan G C x y) :
-  ∀ u ∈ F.val, u ≠ y → (color c G C (x, u)).isSome := by
+theorem fan_colored_edges (x y : Vertex n) (F : Fan C x y) :
+  ∀ u ∈ F.val, u ≠ y → (color C (x, u)).isSome := by
   intro u h1 h2
   rw [← Array.mem_toList_iff] at h1
   have := chain'_rel F.colorAx h1
@@ -39,10 +39,10 @@ theorem fan_colored_edges (x y : Vertex n) (F : Fan G C x y) :
   apply Option.isSome_iff_exists.mpr
   use a; exact Eq.symm ha
 
-def last (F : Fan G C x y) :=
+def last (F : Fan C x y) :=
   F.val.back (by exact Array.size_pos_iff.mpr F.nonemptyAx)
 
-theorem back_neq (F : Fan G C x y) (h : F.val.size > 1) :
+theorem back_neq (F : Fan C x y) (h : F.val.size > 1) :
   F.val.back (by exact Array.size_pos_iff.mpr F.nonemptyAx) ≠ y := by
   simp [← F.firstElemAx, Array.back]
   intro hc
