Vizing/Path/Maximal.lean
@@ -5,7 +5,7 @@ open Graph
 open EdgeColoring
 open Aux
 
-variable {c n : Nat} (G : Graph n) (C : EdgeColoring c G)
+variable {c n : Nat} {G : Graph n} (C : EdgeColoring c G)
 /-
 Function: convert vertex path to edge path
 [a, b, c, d] -> [(a, b), (b, c), (c, d)]
@@ -22,8 +22,7 @@ variable (a b : Color c) (x : Vertex n)
 -- Takes an existing path, extends it using a color d
 def extendPath (d : Color c) (P : List (Vertex n)) (h : P ≠ []) :
   List (Vertex n) :=
-  let u := P.getLast h
-  match (nbhd G u).val.find? (fun v => color c G C (u, v) = d) with
+  match findNborWithColor C (P.getLast h) d with
   | none => P
   | some z => z :: P
 
